Tactics/FunctorReflectionUntyped.v
@@ -1,0 +1,120 @@
+Require Export Control.Functor.
+
+Variables
+  (F : Type -> Type)
+  (F_inst : Functor F)
+  (pure : forall A : Type, A -> F A).
+
+Inductive Exp : Type :=
+    | Var : forall A : Type, A -> Exp
+    | Id : Exp
+    | Comp : Exp -> Exp -> Exp
+    | App : Exp -> Exp -> Exp
+    | Fmap : Exp -> Exp.
+
+Arguments Var {A}.
+
+Inductive type : Type :=
+    | TVar : Type -> type
+    | TArr : type -> type -> type
+    | TF : type -> type.
+
+Fixpoint typeDenote (t : type) : Type :=
+match t with
+    | TVar A => A
+    | TArr t1 t2 => typeDenote t1 -> typeDenote t2
+    | TF t => F (typeDenote t)
+end.
+
+(*
+Fixpoint infer (e : Exp) : type :=
+match e with
+    | @Var A _ => TVar A
+    | 
+end.
+*)
+
+Inductive hasType : Exp -> type -> Type :=
+    | ht_Var :
+        forall (A : Type) (x : A), hasType (Var x) (TVar A)
+    | ht_Id :
+        forall A : type, hasType Id (TArr A A)
+    | ht_Comp :
+        forall (A B C : type) (e1 e2 : Exp),
+          hasType e1 (TArr A B) -> hasType e2 (TArr B C) ->
+            hasType (Comp e1 e2) (TArr A C)
+    | ht_App :
+        forall (A B : type) (e1 e2 : Exp),
+          hasType e1 (TArr A B) -> hasType e2 A ->
+            hasType (App e1 e2) B
+    | ht_Fmap :
+        forall (A B : type) (e : Exp),
+          hasType e (TArr A B) -> hasType (Fmap e) (TArr (TF A) (TF B)).
+
+Hint Constructors hasType.
+
+Function denote {e : Exp} {t : type} (ht : hasType e t) : typeDenote t :=
+match ht with
+    | ht_Var _ x => x
+    | ht_Id _ => id
+    | ht_Comp _ _ _ _ _ e1 e2 => denote e1 .> denote e2
+    | ht_App _ _ _ _ e1 e2 => denote e1 (denote e2)
+    | ht_Fmap _ _ _ e => fmap (denote e)
+end.
+
+Lemma denote_eq {e : Exp} {t : type} (ht : hasType e t) :
+  denote ht =
+  match ht with
+      | ht_Var _ x => x
+      | ht_Id _ => id
+      | ht_Comp _ _ _ _ _ e1 e2 => denote e1 .> denote e2
+      | ht_App _ _ _ _ e1 e2 => denote e1 (denote e2)
+      | ht_Fmap _ _ _ e => fmap (denote e)
+  end.
+Proof.
+  destruct ht; cbn; reflexivity.
+Defined.
+
+Require Import Recdef.
+
+Function simplify (e : Exp) : Exp :=
+match e with
+    | Var x => Var x
+    | Id => Id
+    | Comp e1 e2 =>
+        match simplify e1, simplify e2 with
+            | Id, e2' => e2'
+            | e1', Id => e1'
+            | e1', e2' => Comp e1' e2'
+        end
+    | App e1 e2 =>
+        match simplify e1 with
+            | Id => simplify e2
+            | e1' => App e1' (simplify e2)
+        end
+    | Fmap e' =>
+        match simplify e' with
+            | Id => Id
+            | Comp e1 e2 => Comp (Fmap e1) (Fmap e2)
+            | e'' => Fmap e''
+        end
+end.
+
+Lemma hasType_simplify :
+  forall {e : Exp} {t : type},
+    hasType e t -> hasType (simplify e) t.
+Proof.
+  induction 1; cbn; eauto.
+    inv IHX1; inv IHX2; eauto.
+    inv IHX1; inv IHX2; eauto.
+    inv IHX; eauto.
+Defined.
+
+Lemma denote_simplify :
+  forall {e : Exp} {t : type} (ht : hasType e t),
+    denote (hasType_simplify ht) = denote ht.
+Proof.
+  induction ht.
+    reflexivity.
+    reflexivity.
+Abort.
